src/reflection/FStar.Reflection.NBEEmbeddings.fsti
@@ -27,6 +27,8 @@ module RD = FStar.Reflection.Data
 
 (* Embeddings *)
 val e_bv            : embedding bv
+let e_namedv = e_bv
+
 val e_binder        : embedding binder
 val e_binder_view   : embedding binder_view
 val e_binders       : embedding binders
@@ -48,6 +50,7 @@ val e_letbinding    : embedding letbinding
 val e_lb_view       : embedding lb_view
 val e_sigelt_view   : embedding sigelt_view
 val e_bv_view       : embedding bv_view
+val e_namedv_view   : embedding namedv_view
 val e_exp           : embedding exp
 val e_attribute     : embedding attribute
 val e_attributes    : embedding (list attribute) (* This seems rather silly, but `attributes` is a keyword *)
